update

Licenta.dfy
@@ -12,8 +12,7 @@ function max(p1: int, p2: int): int
 
 function gain(problem: Problem, solution: seq<int>): int
   requires isValidProblem(problem)
-  requires 0 <= |solution| <= problem.numberOfObjects
-  // requires isValidPartialSolution(problem, solution)
+  requires isValidPartialSolution(problem, solution)
 {
   if |solution| == 0 then 0 else computeGain(problem.gains, solution, |solution| - 1)
 }
@@ -61,50 +60,45 @@ predicate isSolution(p: Problem, solution: seq<int>)
 
 predicate isValidPartialSolution(problem: Problem, solution: seq<int>)
 {
-  0 <= |solution| <= problem.numberOfObjects && 
-  forall k :: 0 <= k < |solution| ==> solution[k] == 0 || solution[k] == 1
+  0 <= |solution| <= problem.numberOfObjects && hasOnlyPermittedValues(solution)
 }
 
 predicate isPartialSolution(problem: Problem, solution: seq<int>)
   requires isValidProblem(problem)
-{
-  isValidPartialSolution(problem, solution) && 
-  weight(problem, solution) < problem.knapsackCapacity
+  requires isValidPartialSolution(problem, solution)
+{ 
+  weight(problem, solution) <= problem.knapsackCapacity
 }
 
 ghost predicate isPartialSolutionOfCoordinates(p: Problem, profits: seq<seq<int>>, partialProfits: seq<int>, dim: int, weight: int)
   requires isValidProblem(p)
+  requires 0 <= weight <= p.knapsackCapacity && 0 <= weight < |partialProfits|
+  requires |profits| == 0 ==> dim == 0
+  requires |profits| == 1 ==> dim == 1
+  requires |profits| > 1 ==> dim == |profits|
 {
-  checkCaseOne(p, profits, partialProfits, dim, weight) || checkCaseTwo(p, profits, partialProfits, dim, weight) ||
-  checkCaseThree(p, profits, partialProfits, dim, weight)
+  forall k :: 0 <= k < |partialProfits| ==> 
+  (existsGain(p, partialProfits[k]) && existsPartialWeigth(p, weight))
 }
 
-ghost predicate checkCaseOne(p: Problem, profits: seq<seq<int>>, partialProfits: seq<int>, dim: int, weight: int)
-{
-  |profits| == 0 && dim == 0 && 0 <= weight <= p.knapsackCapacity
-  && forall k :: 0 <= k < |partialProfits| ==> partialProfits[k] == 0
-}
-
-ghost predicate checkCaseTwo(p: Problem, profits: seq<seq<int>>, partialProfits: seq<int>, dim: int, weight: int)
+ghost predicate isPartialSolutionOfProfit(p: Problem, profits: seq<seq<int>>, dim: int, weight: int)
   requires isValidProblem(p)
+  requires |profits| == 0 || (0 <= dim < |profits| && 0 <= dim < p.numberOfObjects + 1 &&
+   0 <= weight < |profits[dim]| && 0 <= weight < p.knapsackCapacity + 1)
 {
-  |profits| == 1 ==> (dim == 1 && 0 <= weight <= p.knapsackCapacity && 0 <= weight < |partialProfits|
-  && existsGain(p, partialProfits[weight]))
+   0 <= dim < |profits| && existsGain(p, profits[dim][weight]) && existsPartialWeigth(p, weight)
 }
-
-ghost predicate checkCaseThree(p: Problem, profits: seq<seq<int>>, partialProfits: seq<int>, dim: int, weight: int)
-  requires isValidProblem(p)
-{
-  |profits| > 1 ==> (dim == |profits| && 0 <= weight <= p.knapsackCapacity && 0 <= weight < |partialProfits|
-  && existsGain(p, partialProfits[weight]))
-}
-
-
 
 ghost predicate existsGain(p: Problem, profit: int)
   requires isValidProblem(p)
 {
   exists sol : seq<int> :: isValidPartialSolution(p, sol) && gain(p, sol) == profit
+}
+
+ghost predicate existsPartialWeigth(p: Problem, partialWeight: int)
+  requires isValidProblem(p)
+{
+  exists sol : seq<int> :: isValidPartialSolution(p, sol) && weight(p, sol) == partialWeight
 }
 
 ghost predicate isOptimalSolution(problem: Problem, solution: seq<int>)
@@ -116,7 +110,7 @@ ghost predicate isOptimalSolution(problem: Problem, solution: seq<int>)
     gain(problem, solution) >= gain(problem, s)))
 }
 
-predicate hasOnlyRequiredValues(solution: seq<int>)
+predicate hasOnlyPermittedValues(solution: seq<int>)
 {
   forall k :: 0 <= k < |solution| ==> solution[k] == 0 || solution[k] == 1
 }
@@ -131,12 +125,13 @@ method addSequence(existingSeq: seq<seq<int>>, newSeq: seq<int>, c: int) returns
 
 method getMaximProfit(p: Problem) returns (solution: seq<int>)
   requires isValidProblem(p)
-  ensures hasOnlyRequiredValues(solution)
-  // ensures isValidSolution(p, solution)
   // ensures isSolution(p, solution)
+  ensures isValidPartialSolution(p, solution)
+  
 {
     var profits := []; 
     var maximProfit := 0;
+    var partialProfits := [];
 
     var i := 0;
     while i <= p.numberOfObjects 
@@ -144,17 +139,15 @@ method getMaximProfit(p: Problem) returns (solution: seq<int>)
       invariant 0 <= i <= p.numberOfObjects + 1
       invariant forall k :: 0 <= k < i ==> |profits[k]| == p.knapsackCapacity + 1
       invariant 0 <= |profits| <= p.numberOfObjects + 1
-      // invariant forall x :: 0 <= x < i ==> forall y :: 0 <= y <= p.knapsackCapacity ==> 
-      //   isPartialSolutionOfProfit(p, profits, x, y)
+      // invariant |profits| > 0 ==> (forall x :: 0 <= x < i ==> forall y :: 0 <= y <= p.knapsackCapacity ==> 
+      //   isPartialSolutionOfProfit(p, profits, x, y))
     {
-        var partialProfits := getPartialProfits(p, profits, i);
+        partialProfits := getPartialProfits(p, profits, i);
         profits := addSequence(profits, partialProfits, p.knapsackCapacity + 1);
         i := i + 1; 
     }
-
+    
     maximProfit := profits[p.numberOfObjects][p.knapsackCapacity];
-    assert (|profits| == p.numberOfObjects + 1);
-
     solution := getKnapsackObjects(p, profits);
 }
 
@@ -165,8 +158,7 @@ method getPartialProfits(p: Problem, profits: seq<seq<int>>, i: int) returns (pa
   requires forall k :: 0 <= k < i ==> |profits[k]| == p.knapsackCapacity + 1
   ensures |partialProfits| == p.knapsackCapacity + 1
   ensures 0 <= |profits| <= p.numberOfObjects + 1
-  // ensures isSolution(p, solution)
-  ensures forall y :: 0 <= y < |partialProfits| ==> (isPartialSolutionOfCoordinates(p, profits, partialProfits, i, y))
+  // ensures forall y :: 0 <= y < |partialProfits| ==> (isPartialSolutionOfCoordinates(p, profits, partialProfits, i, y))
 {
         partialProfits := [];
         var j := 0;
@@ -175,9 +167,12 @@ method getPartialProfits(p: Problem, profits: seq<seq<int>>, i: int) returns (pa
           invariant 0 <= j <= p.knapsackCapacity + 1
           invariant 0 <= |profits| <= p.numberOfObjects + 1
           invariant |partialProfits| == j
-          invariant |partialProfits| > 0 ==> 
-        (forall y :: 0 <= y < |partialProfits| ==> (isPartialSolutionOfCoordinates(p, profits, partialProfits, i, y)))
+        //   invariant |partialProfits| > 0 ==> 
+        // (forall y :: 0 <= y < |partialProfits| ==> (existsGain(p, partialProfits[y])))
+        // invariant |partialProfits| > 0 ==> 
+        // (forall y :: 0 <= y < |partialProfits| ==> (existsPartialWeigth(p, y)))
         {
+          // assert isPartialSolutionOfCoordinates(p, profits, partialProfits, 0, 0);
           if i == 0 || j == 0 {
               partialProfits := partialProfits + [0];
           } else {
@@ -191,67 +186,29 @@ method getPartialProfits(p: Problem, profits: seq<seq<int>>, i: int) returns (pa
         }
 }
 
-// method getKnapsackObjects(p: Problem, profits: seq<seq<int>>) returns (solution: seq<int>)
-//   requires isValidProblem(p)
-//   requires |profits| == p.numberOfObjects + 1
-//   requires forall k :: 0 <= k <= p.numberOfObjects ==> |profits[k]| == p.knapsackCapacity + 1
-//   ensures isValidSolution(p, solution)
-// {
-//     solution := [];
-//     var i := p.numberOfObjects;
-//     var j := p.knapsackCapacity;
-
-//     while i > 0 && j >= 0
-//       invariant 0 <= i <= p.numberOfObjects
-//       invariant 0 <= j <= p.knapsackCapacity
-//       invariant |solution| == p.numberOfObjects - i
-//       invariant isPartialSolution(p, solution)
-//       decreases i
-//       decreases j
-//     {
-//       if profits[i][j] == profits[i - 1][j] {
-//         solution := [0] + solution;
-//         i := i - 1;
-//       } else { 
-//         solution := [1] + solution;
-//         i := i - 1;
-//         if j - p.weights[i] >= 0 {
-//           j := j - p.weights[i];
-//         }
-//       }
-//     }
-// }
-
-predicate solIncreasedByOne(oldSol: seq<int>, newSol: seq<int>)
-{
-  |newSol| > 0 ==> |newSol| == |oldSol| + 1
-}
-
 method getKnapsackObjects(p: Problem, profits: seq<seq<int>>) returns (solution: seq<int>)
     requires isValidProblem(p)
-    requires 0 <= |profits| <= p.numberOfObjects + 1
-    requires forall k :: 0 <= k < |profits| ==> |profits[k]| == p.knapsackCapacity + 1
     requires |profits| <= |p.weights| + 1
-    ensures hasOnlyRequiredValues(solution)
-    ensures |profits| > 0 ==> 0 <= |solution| < |profits|
+    requires forall k :: 0 <= k < |profits| ==> |profits[k]| == p.knapsackCapacity + 1
+    ensures hasOnlyPermittedValues(solution)
+    ensures isValidPartialSolution(p, solution)
 {
     solution := [];
     var i := |profits| - 1;
     var j := p.knapsackCapacity;
-    var oldSol := solution;
-
     while i > 0 && j >= 0
       invariant -1 <= i <= |profits| - 1
       invariant -1 <= i <= |p.weights|
       invariant 0 <= j <= p.knapsackCapacity
-      invariant |profits| > 0 ==> (|solution| < |profits| - i  && 0 <= |solution| < |profits|)
-      invariant |profits| > 0 ==> 0 <= |solution| < |profits|
-      // invariant isPartialSolution(p, solution)
-      invariant hasOnlyRequiredValues(solution)
+      invariant |profits| > 0 ==> (|solution| < |profits| - i  && 0 <= |solution| <= |profits|)
+      invariant hasOnlyPermittedValues(solution)
+      invariant isValidPartialSolution(p, solution)
+      // invariant forall y :: 0 <= y < |solution| ==> (weight(p, solution) <= p.knapsackCapacity)
+      invariant isPartialSolution(p, solution)
       decreases i
       decreases j
     {
-      oldSol := solution;
+      // assert isPartialSolution(p, solution);
       if profits[i][j] == profits[i - 1][j] {
         solution := [0] + solution;
         i := i - 1;
@@ -272,6 +229,6 @@ method Main()
     var solution := getMaximProfit(problem);
 
     print "Maxim profit: ";
-    // print gain(problem, solution);
+    print gain(problem, solution);
     print "\n";
 }
